Semantics/I_Seq_Semantics.thy
@@ -1,0 +1,27 @@
+theory I_Seq_Semantics
+  imports I_Semantics Seq_Semantics
+begin
+
+locale I_Seq_Semantics = I_Semantics_Sig + Seq_Semantics_Sig
+
+sublocale I_Semantics \<subseteq> Base_Next_Semantics
+  where base_sem = i_base_sem
+  done
+
+
+sublocale I_Seq_Semantics \<subseteq> I_Semantics
+  where i_sem = i_sem
+  done
+
+sublocale I_Seq_Semantics \<subseteq> Seq_Semantics
+  where seq_sem = seq_sem
+  done
+
+
+print_locale! I_Seq_Semantics
+
+sublocale I_Seq_Semantics \<subseteq> Gensyn_Semantics
+  where base_sem = i_base_sem
+    and rec_sem = seq_rec_sem
+
+end
