Semantics/Seq_Semantics.thy
@@ -1,0 +1,73 @@
+theory Seq_Semantics imports "Gensyn_Semantics_Fuse2" "../Syntax/Syn_Seq"
+begin
+
+locale Seq_Semantics_Sig =
+  fixes seq_sem :: "'g \<Rightarrow> 'sq \<Rightarrow> 'mstate \<Rightarrow> 'mstate \<Rightarrow> bool"
+
+
+
+locale Seq_Semantics = Seq_Semantics_Sig 
+begin
+
+print_context
+
+(* problem - this specifies next behavior for all base nodes
+   is that really what we want? it may actually be, i'm just not sure. *)
+(* another option is to just have this encapsulate descending into a base
+   node and handling "next" elsewhere, perhaps at the "elle" level... *)
+(* a third option is to only use "unhandled" cases *)
+(* another way to get at this: what should the hierarchy look like? *)
+(* hierarchy: can we worry about it later? *)
+inductive seq_rec_sem :: "'a \<Rightarrow> ('b, 'xb, 'xa) syn_seq \<Rightarrow> 'c \<Rightarrow> 'c \<Rightarrow>
+  childpath \<Rightarrow> ('bs, ('b, 'xb, 'xa) syn_seq, 'a) gensyn \<Rightarrow> ('xr) gs_result \<Rightarrow> bool" where
+"seq_sem g s m m' \<Longrightarrow> seq_rec_sem g (LSeq s) m m' cp sk (GRPath (cp@[0]))"
+
+end
+
+(* sublocale Seq_Semantics \<subseteq> Gensyn_Semantics
+  ...
+*)
+
+locale Base_Next_Semantics = Gensyn_Semantics_Base_Sig 
+begin
+inductive base_sem_next ::
+    "'a \<Rightarrow> 'b \<Rightarrow> 'c \<Rightarrow> 'c \<Rightarrow> childpath \<Rightarrow>
+            ('b, 'd, 'a) gensyn \<Rightarrow>
+                 ('e) gs_result \<Rightarrow> bool"
+    where
+"base_sem g b m m' cp t GRUnhandled \<Longrightarrow>
+ gensyn_cp_next t cp = Some cp' \<Longrightarrow>
+  base_sem_next g b m m' cp t (GRPath cp')"
+| "base_sem g b m m' cp t GRUnhandled \<Longrightarrow>
+  gensyn_cp_next t cp = None \<Longrightarrow>
+  base_sem_next g b m m' cp t (GRDone)"
+| "base_sem g b m m' cp t res \<Longrightarrow>
+  base_sem_next g b m m' cp t res"
+
+end
+
+(*
+locale Seq_Next_Semantics = Seq_Semantics +
+  fixes base_sem :: "'g \<Rightarrow> 'b \<Rightarrow> 'mstate \<Rightarrow> 'mstate \<Rightarrow> childpath \<Rightarrow>
+                 ('b, ('sq, 'xbr, 'xar) syn_seq, 'g) gensyn \<Rightarrow>
+                     ('xrs) gs_result \<Rightarrow> bool"
+
+begin
+
+inductive base_sem_next ::
+    "'g \<Rightarrow> 'b \<Rightarrow> 'mstate \<Rightarrow> 'mstate \<Rightarrow> childpath \<Rightarrow>
+            ('b, ('sq, 'xbr, 'xar) syn_seq, 'g) gensyn \<Rightarrow>
+                 ('xrs) gs_result \<Rightarrow> bool"
+    where
+"base_sem g b m m' cp t GRUnhandled \<Longrightarrow>
+ gensyn_cp_next t cp = Some cp' \<Longrightarrow>
+  base_sem_next g b m m' cp t (GRPath cp')"
+| "base_sem g b m m' cp t GRUnhandled \<Longrightarrow>
+  gensyn_cp_next t cp = None \<Longrightarrow>
+  base_sem_next g b m m' cp t (GRDone)"
+| "base_sem g b m m' cp t res \<Longrightarrow>
+  base_sem_next g b m m' cp t res"
+
+end
+*)
+end
